src/Syntax.v
@@ -2,12 +2,14 @@ From Coq Require Import Unicode.Utf8.
 From Coq Require Import Strings.String.
 Local Open Scope Z_scope.
 Require Import ZArith.
+Require Import Maps.
 Require Import Hints.
 
 Inductive type :=
 | Type_Num
 | Type_Bool
-| Type_Fun (e1 e2 : type) : type
+| Type_Fun (t₁ t₂ : type)
+| Type_Rec (m : @Maps.map type)
 .
 
 
@@ -21,7 +23,14 @@ Inductive expr :=
 | E_Let (x : string) (e1 e2 : expr)
 | E_Num (z : Z)
 | E_Minus (e1 e2 : expr)
+| E_Rec (fields : @Maps.map expr)
+| E_Access (e : expr) (field : string)
 .
+
+(* 
+  Les records sont des map `nom du champ -> expr`
+  Une paire de type A × B peut être représentée comme un record { first : A, second : B }
+*)
 
 
 
@@ -35,6 +44,9 @@ Inductive value : expr -> Prop :=
         (t : type) 
         (e : expr), 
     value (E_Fun x t e)
+| V_Rec :
+  ∀ m,
+  value (E_Rec m)
 .
 
 Hint Constructors type : local_hints.
