src/Types.v
@@ -8,41 +8,57 @@ Definition context := @Maps.map type.
 Definition empty := @Maps.empty type.
 
 Inductive has_type : context -> expr -> type -> Prop := 
-    | T_Var: ∀ Γ x t, 
-                Γ ? x = Some t -> 
-                has_type Γ (E_Var x) t
+    | T_Var: 
+        ∀ Γ x t, 
+        Γ ? x = Some t -> 
+        has_type Γ (E_Var x) t
 
-    | T_Fun: ∀ Γ x t1 e t2,
-                has_type (x |-> t1; Γ) e t2 ->
-                has_type Γ (E_Fun x t1 e) (Type_Fun t1 t2)
-    | T_App: ∀ Γ e1 e2 t1 t2, 
-                has_type Γ e2 t1 -> 
-                has_type Γ e1 (Type_Fun t1 t2) ->
-                has_type Γ (E_App e1 e2) t2
+    | T_Fun: 
+        ∀ Γ x t1 e t2,
+        has_type (x |-> t1; Γ) e t2 ->
+        has_type Γ (E_Fun x t1 e) (Type_Fun t1 t2)
 
-    | T_True: ∀ Γ, 
-                has_type Γ E_True Type_Bool
+    | T_App: 
+        ∀ Γ e1 e2 t1 t2, 
+        has_type Γ e2 t1 -> 
+        has_type Γ e1 (Type_Fun t1 t2) ->
+        has_type Γ (E_App e1 e2) t2
+
+    | T_True: 
+        ∀ Γ, 
+        has_type Γ E_True Type_Bool
                 
-    | T_False: ∀ Γ, 
-                has_type Γ E_False Type_Bool
+    | T_False: 
+        ∀ Γ, 
+        has_type Γ E_False Type_Bool
 
-    | T_If: ∀ Γ e1 e2 e3 t, 
-                has_type Γ e1 Type_Bool -> 
-                has_type Γ e2 t -> 
-                has_type Γ e3 t -> 
-                has_type Γ (E_If e1 e2 e3) t 
+    | T_If: 
+        ∀ Γ e1 e2 e3 t, 
+        has_type Γ e1 Type_Bool -> 
+        has_type Γ e2 t -> 
+        has_type Γ e3 t -> 
+        has_type Γ (E_If e1 e2 e3) t 
 
-    | T_Let : ∀ Γ x e1 e2 t1 t2, 
-                has_type Γ e1 t1 -> 
-                has_type (x |-> t1; Γ) e2 t2 -> 
-                has_type Γ (E_Let x e1 e2) t2
+    | T_Let : 
+        ∀ Γ x e1 e2 t1 t2, 
+        has_type Γ e1 t1 -> 
+        has_type (x |-> t1; Γ) e2 t2 -> 
+        has_type Γ (E_Let x e1 e2) t2
 
-    | T_Num : ∀ Γ z, has_type Γ (E_Num z) Type_Num 
+    | T_Num : 
+        ∀ Γ z, 
+        has_type Γ (E_Num z) Type_Num 
 
-    | T_Minus : ∀ Γ e1 e2, 
-                has_type Γ e1 Type_Num ->
-                has_type Γ e2 Type_Num ->
-                has_type Γ (E_Minus e1 e2) Type_Num 
+    | T_Minus : 
+        ∀ Γ e1 e2, 
+        has_type Γ e1 Type_Num ->
+        has_type Γ e2 Type_Num ->
+        has_type Γ (E_Minus e1 e2) Type_Num 
+    
+    | T_Rec : 
+        ∀ Γ m_fields m_types,
+        Maps.same_bindings m_fields m_types -> 
+        has_type Γ (E_Rec m_fields) (Type_Rec m_types)
     .
 
 Hint Constructors has_type : local_hints.
